@@ -42,4 +42,5 @@ public inductive BvTerm (v: VarWidths): Nat → Type where
   | BinaryNormal: {w: Nat} → BvTerm v w → BvTerm v w → BiNormalOp → BvTerm v w
   | BinaryReduction: {w: Nat} → BvTerm v w → BvTerm v w → BiReductionOp → BvTerm v 1
   | Extension: {w:Nat} → BvTerm v w → (m: Nat) → ExtOp → BvTerm v m
+  | Ite: {w: Nat} → BvTerm v 1 → BvTerm v w → BvTerm v w → BvTerm v w
 deriving Repr, Nonempty
